---
banner: "![[maths.jpg]]"
---
# Trigonometric Identities 
$\DeclareMathOperator{cosec}{cosec}$
> [!Tip] Identities 
> - $$\tan^2\theta+1\equiv \frac{1}{\cos^2\theta}$$
> - $$1+\cot^2\theta\equiv \cosec^2\theta$$
> ---
> - $$\tan^2\theta=sec^2\theta-1$$
> - $$\cot^2\theta\equiv \cosec^2\theta-1$$

> [!Example]- Solve $\frac{\tan^2x}{\sec x}=\sec x-\cos x$
> - $LHS=\frac{sec^2x-1}{\sec x}$
> - $\frac{\sec^2x}{\sec x}-\frac{1}{\sec x}$
> - $\sec x-\cos x$
> - $=RHS$

> [!Example]- Prove the identity $\frac{\tan^2x}{\sec x+1}\equiv \sec x-\cos^2x-\sin^2x$
> - $LHS=\frac{\sec^2x-1}{\sec x+1}$
> - $\frac{\cancel{ (\sec x+1) }(\sec x-1)}{\cancel{ \sec x+1 }}$
> - $\sec x-1$
> - $\sec x-(\sin^2x+\cos^2x)$
> - $\sec x-\sin^2x-\cos^2x$
> - $=RHS$

> [!Example]- Prove the identity $\cosec^4\theta-\cot^4\theta\equiv\frac{1+\cos^2\theta}{1-\cos^2\theta}$
> - $LHS=\cosec^4\theta-\cot^4\theta$
> - $=(\cosec^2\theta+\cot^2\theta)(\cosec^2\theta-\cot^2\theta)$
> - $=\cosec^2\theta+\cot^2\theta$
> - $=\frac{1}{\sin^2\theta}+\frac{\cos^2\theta}{\sin^2\theta}$
> - $=\frac{1}{\sin^2\theta}+\frac{\cos^2\theta}{\sin^2\theta}$
> - $=\frac{1+\cos^2\theta}{\sin^2\theta}$
> - $=\frac{1+\cos^2\theta}{1-\cos^2\theta}=RHS$
