---
banner: "![[maths.jpg]]"
---
# Addition Formulae 
$\DeclareMathOperator{cosec}{cosec}$
> [!Tip] The Formulae 
> - $$\sin(A+B)\equiv\sin A\cos B+\cos A\sin B$$
> - $$\cos(A+B)\equiv \cos A\cos B-\sin A\sin B$$
> - $$\tan(A+B)\equiv \frac{\tan A+\tan B}{1-\tan A\tan B}$$
> - $$\sin(A-B)\equiv\sin A\cos B-\cos A\sin B$$
> - $$\cos(A-B)\equiv \cos A\cos B+\sin A\sin B$$
> - $$\tan(A-B)\equiv \frac{\tan A-\tan B}{1+\tan A\tan B}$$

> [!Example]- Show using the formula for $\sin(A-B)$ that $\sin(15^{\circ})=\frac{\sqrt{ 6 }-\sqrt{ 2 }}{4}$
> - $\sin(A-B)=\sin A\cos B-\cos A\sin B$
> - $\sin(45-30)=\sin45\cos30-\sin30\cos45$
> - $=\left( \frac{\sqrt{ 2 }}{2}\times \frac{\sqrt{ 3 }}{2} \right)-\left( \frac{1}{2}\times \frac{\sqrt{ 2 }}{2} \right)$
> - $=\frac{\sqrt{ 6 }}{4}-\frac{\sqrt{ 2 }}{4}$
> - $=\frac{\sqrt{ 6 }-\sqrt{ 2 }}{4}$

> [!Example]- Show that $\cos3\theta=4\cos^3\theta-3\cos\theta$
> - $LHS=\cos3\theta=\cos(\theta+2\theta)$
> - $=\cos\theta \cos2\theta-\sin\theta \sin2\theta$
> - $=\cos\theta(2\cos^2\theta-1)-\sin\theta(2\sin\theta \cos\theta)$
> - $=2\cos^3\theta-\cos\theta-2\sin^2\theta \cos\theta$
> - $=2\cos^3\theta-\cos\theta-2(1-\cos^2\theta)$
> - $=4\cos^3\theta-3\cos\theta=RHS$

