---
banner: "![[furthermaths.jpg]]"
---
# Proving Statements involving Matrices

> [!Example]- Prove that $\begin{pmatrix}1 & -1 \\ 0 & 2\end{pmatrix}^n=\begin{pmatrix}1 & 1-2^n \\ 0 & 2^n\end{pmatrix}$ for all $n\in \natural$
> - When n=1, LHS = $\begin{pmatrix}1 & -1  \\ 0 & 2\end{pmatrix}^1=\begin{pmatrix}1 & -1 \\ 0 & 2\end{pmatrix}$
> - Assume holds true for $n=k$ $\begin{pmatrix}1 & -1 \\ 0 & 2\end{pmatrix}^k$
>   ![[PXL_20230313_093825438.jpg|400]]
>  - $\therefore$ holds true for $n=k+1$
>  - Since true for $n=1$ and true for $n=k$, true for $n=k+1$ and therefore true for all $n$.

