---
banner: "![[furthermaths.jpg]]"
---
# Expressions relating to the Roots of Polynomials#

> [!Info] Rewriting root equations as reciprocals
> $$\frac{1}{\alpha}+\frac{1}{\beta}=\frac{\alpha+\beta}{\alpha\beta}$$
> $$\frac{1}{\alpha}+\frac{1}{\beta}+\frac{1}{\gamma}=\frac{\alpha\beta+\alpha\gamma+\beta\gamma}{\alpha+\beta+\gamma}$$
> $$\frac{1}{\alpha}+\frac{1}{\beta}+\frac{1}{\gamma}+\frac{1}{\delta}=\frac{\alpha\beta\gamma+\beta\gamma\delta+\alpha\gamma\delta+\alpha\beta\delta}{\alpha\beta\gamma\delta}$$

> [!Info] Sum of the squares equations
> Quadratic: $$ \alpha^2+\beta^2=(\alpha+\beta)^2-2\alpha\beta$$
> Cubic: $$\alpha^2+\beta^2+\gamma^2=(\alpha+\beta+\gamma)^2-2(\alpha\beta+\beta\gamma+\alpha\gamma)$$
> Quartic: $$\alpha^2+\beta^2+\gamma^2+\delta^2=(\alpha+\beta+\gamma+\delta)^2-2(\alpha\beta+\alpha\gamma+\alpha\delta+\beta\gamma+\beta\delta+\gamma\delta)$$

> [!Info] Sum of the cubes equations
> Quadratic: $$\alpha^3+\beta^3=(\alpha+\beta)^3-3\alpha\beta(\alpha+\beta)$$
> Cubic: $$\alpha^3+\beta^3+\gamma^3=(\alpha+\beta+\gamma)^3-3(\alpha+\beta+\gamma)(\alpha\beta+\beta\gamma+\alpha\gamma)+3\alpha\beta\gamma$$

> [!Info] Rules for products of powers
> Quadratic: $$\alpha^n\times\beta^n=(\alpha\beta)^n$$
> Cubic: $$\alpha^n\times\beta^n\times\gamma^n=(\alpha\beta\gamma)^n$$
> Quartic: $$\alpha^n\times\beta^n\times\gamma^n\times\delta^n=(\alpha\beta\gamma\delta)^n$$



