---
banner: "![[furthermaths.jpg]]"
---
# Linear Transformations of Roots

> [!Info] Linear Transformation of Roots by relationship between roots and coefficients
> - If we have the equation: $x^2-3x-10=0$ which has the roots $\alpha$ and $\beta$, what is the equation of the polynomial with roots $\alpha-1$ and $\beta-1$?
> - $\alpha+\beta=\frac{3}{1}=3$
> - $\alpha\beta=\frac{c}{a}=-\frac{10}{1}=-10$
> - We know that $\alpha-1+\beta-1=-\frac{b}{a}$
> - $\alpha+\beta-2=-\frac{b}{a}$
> - Since $\alpha+\beta=3$:
> - $-\frac{b}{a}=3-2=1$
> 
>   We have the first value!
>   
>   - $(\alpha-1)(\beta-1)=\frac{c}{a}$
>   - $\alpha\beta-(\alpha+\beta)+1=\frac{c}{a}$
>   - $\frac{c}{a}=-10-3+1=-12$
>- Therefore our new equation is $x^2+x-12$
>- This is a **VERY** long winded approach, therefore it would be better to use a substitution.

> [!Info] Linear Transformation of Roots using substitution
> - If we have the equation: $x^2-3x-10=0$ which has the roots $\alpha$ and $\beta$, what is the equation of the polynomial with roots $\alpha-1$ and $\beta-1$?
> - $W=x-1$
> - $(W-1)^2-3(W-1)-10=0$
> - $W^2+2W+1-3W-3-10=0$
> - $W^2-W-12$
> - New function is: $x^2-x-12=0$

> [!Example]- Using subtitution on a quartic.
> - Original polynomial = $x^4-3x^3+15x+1=0$
> - $W=2x+1$
> - $x=\frac{W-1}{2}$
> - Transformed polynomial = $\frac{(W-1)^4}{16}-\frac{3(W-1)^3}{8}+\frac{15(W-1)}{2}+1=0$
> - Times all by 16
> - Expand out
> - To be done later!